veric/initial_world.v
@@ -108,12 +108,14 @@ case_eq (Share.split Share.top); intros; simpl.
 eapply nonemp_split_neq1; eauto.
 Qed.
 
-Lemma dec_pure: forall r, {exists k, exists pp, r = PURE k pp}+{core r = NO Share.bot bot_unreadable}.
+Lemma dec_pure: forall r, {exists k, exists pp, r = PURE k pp}+
+  {core r = NO Share.bot bot_unreadable \/ exists m, core r = GHOST (core m)}.
 Proof.
  destruct r.
- right; apply core_NO.
- right; apply core_YES.
+ right; left; apply core_NO.
+ right; left; apply core_YES.
  left; eauto.
+ right; right; eexists; apply core_GHOST.
 Qed.
 
 Lemma store_init_data_list_lem:
@@ -161,6 +163,7 @@ assert (Hv: CompCert_AV.valid (res_option oo f)).
   rewrite core_NO in H5; inv H5.
   rewrite core_YES in H5; inv H5.
   rewrite core_PURE in H5; inv H5.
+  rewrite core_GHOST in H5; inv H5.
 destruct (remake_rmap f Hv (level w)) as [m2 [? ?]]; clear Hv.
 intros; unfold f, no_preds; simpl; intros; repeat if_tac; auto.
 left. exists (core w). rewrite core_resource_at. rewrite level_core.  auto.
@@ -229,6 +232,9 @@ rewrite core_YES.
 destruct (access_at m (b', z')); try destruct p0; try constructor; auto.
 destruct IOK2 as [? [? ?]].
 rewrite H2. rewrite core_PURE; constructor.
+destruct IOK2 as [? [? ?]].
+rewrite H2. rewrite core_GHOST; constructor.
+apply join_comm, core_unit.
 
 * (**** case 2 of 3 ****)
 intro loc.
@@ -262,7 +268,7 @@ assert (AV.valid  (res_option oo (fun loc => if adr_range_dec (b,lo) (hi-lo) loc
 apply VAL_valid; unfold compose; intros.
 if_tac in H1. inv H1; eauto.
 elimtype False; revert H1; clear; rewrite <- core_resource_at.
-destruct (w @ l); simpl; [rewrite core_NO | rewrite core_YES | rewrite core_PURE]; intro H; inv H.
+destruct (w @ l); simpl; [rewrite core_NO | rewrite core_YES | rewrite core_PURE | rewrite core_GHOST]; intro H; inv H.
 destruct (make_rmap _ H1 (level w)) as [phi [? ?]].
 extensionality loc; unfold compose; if_tac.
 unfold resource_fmap. f_equal.
@@ -342,6 +348,11 @@ rewrite core_PURE.
 destruct (IOK (b',z')).
 rewrite H0 in H3. destruct H3 as [? [? ?]].
 rewrite H4. constructor.
+rewrite core_GHOST.
+destruct (IOK (b',z')).
+rewrite H0 in H3. destruct H3 as [? [? ?]].
+rewrite H4. constructor.
+apply join_comm, core_unit.
 unfold contents_at; inv H; simpl; auto.
 rewrite PMap.gso; auto.
 unfold access_at; inv H; simpl; auto.
@@ -1355,7 +1366,6 @@ destruct f; auto.
 f_equal.
 simpl.
 f_equal.
-change compcert_rmaps.R.rmap with rmap in *.
 rewrite lev'.
 unfold initial_core.
 rewrite level_make_rmap.
@@ -1387,7 +1397,7 @@ Proof.
   unfold inflate_initial_mem; simpl.
   match goal with |- context [ proj1_sig ?a ] => destruct a as (phi & lev & E) end; simpl.
   unfold inflate_initial_mem' in E.
-  unfold compcert_rmaps.R.resource_at in E.
+  unfold resource_at in E.
   unfold no_locks, "@"; intros.
   rewrite E.
   destruct (access_at m addr); try (split; congruence).
@@ -1443,7 +1453,6 @@ Proof.
   rewrite <-approx_oo_approx' with (n' := n) at 3; try omega.
   rewrite <-approx'_oo_approx with (n' := n) at 4; try omega.
   rewrite <-fmap_comp. unfold compose.
-  change compcert_rmaps.R.approx with approx.
   rewrite E.
   reflexivity.
 Qed.
@@ -1473,7 +1482,7 @@ Proof.
   unfold inflate_initial_mem; simpl.
   match goal with |- context [ proj1_sig ?a ] => destruct a as (phi & lev & E) end; simpl.
   unfold inflate_initial_mem' in E.
-  unfold compcert_rmaps.R.resource_at in E.
+  unfold resource_at in E.
   intros b fsig cc A P Q FAT.
   unfold func_at'' in *.
   rewrite level_initial_core in lev.
@@ -1490,7 +1499,7 @@ Proof.
     destruct (access_at m (b, 0)) as [[]|]; simpl in E2; try congruence.
     set (r := proj1_sig _ _) in FAT at 2.
     destruct (proj1_sig (snd (unsquash (initial_core (Genv.globalenv prog) G n))) (b, 0))
-      as [t | t p k p0 | k p] eqn:E'''; simpl in E2; try congruence.
+      as [t | t p k p0 | k p | g] eqn:E'''; simpl in E2; try congruence.
     subst r.
     injection FAT as -> ->; f_equal. subst pp. f_equal.
     simpl. f_equal.
