veric/juicy_mem_lemmas.v
@@ -112,6 +112,11 @@ elimtype False.
 eapply necR_PURE in H1.
 2: constructor 1; eassumption.
 congruence.
+intros.
+elimtype False.
+eapply necR_GHOST in H1.
+2: constructor 1; eassumption.
+congruence.
 Qed.
 
 Lemma preds_fmap_NoneP_approx: forall pp lev1 lev2,
@@ -156,6 +161,9 @@ constructor 1; auto.
 apply (necR_PURE w phi') in H1.
 rewrite H1 in ACCESS; auto.
 constructor 1; auto.
+apply (necR_GHOST w phi') in H1.
+rewrite H1 in ACCESS; auto.
+constructor 1; auto.
 assert (max_access_cohere m w).
 intro loc; specialize (MAXA loc).
 case_eq (w @ loc); intros; auto.
@@ -164,6 +172,9 @@ apply (necR_YES w phi') in H2.
 rewrite H2 in MAXA; auto.
 constructor 1; auto.
 apply (necR_PURE w phi') in H2.
+rewrite H2 in MAXA; auto.
+constructor 1; auto.
+apply (necR_GHOST w phi') in H2.
 rewrite H2 in MAXA; auto.
 constructor 1; auto.
 assert (alloc_cohere m w).
@@ -196,6 +207,7 @@ rewrite Hacc.
 clear - H1.
 simpl.
 unfold perm_of_sh. rewrite if_true by auto. if_tac; constructor.
+contradiction.
 contradiction.
 Qed.
 
@@ -589,6 +601,7 @@ exists sh, r.
 destruct (H1 _ _ _ _ _ H8); subst.
 f_equal.
 inv PERM.
+inv PERM.
 Qed.
 
 Lemma core_load_load: forall ch b ofs v m,
@@ -925,6 +938,7 @@ Focus 2.
   destruct (m_phi j @ (b0,ofs0)).
   rewrite core_NO in H0; inv H0. rewrite core_YES in H0; inv H0.
   rewrite core_PURE in H0. inversion H0. subst k0 p0; constructor.
+  rewrite core_GHOST in H0; inv H0.
   rename H6 into Hm1.
  clear H0.
 destruct (free_nadr_range_eq _ _ _ _ _ _ _ n H) as [H0 H10].
@@ -941,6 +955,21 @@ destruct (free_nadr_range_eq _ _ _ _ _ _ _ n H) as [H0 H10].
   do 2 rewrite core_resource_at.  unfold Join_rmap in *;  unfold Sep_rmap in  *; congruence.
   rewrite Hm1 in H. rewrite H6 in H.
   rewrite core_PURE in H. rewrite core_NO in H; inv H.
+
+  elimtype False.
+  clear - H2 Hm1 H0 H6.
+  assert (core (m1 @ (b0,ofs0)) = core (m_phi j @ (b0,ofs0))).
+  do 2 rewrite core_resource_at.  unfold Join_rmap in *;  unfold Sep_rmap in  *; congruence.
+  rewrite Hm1 in H. rewrite H6 in H.
+  rewrite core_GHOST in H. rewrite core_NO in H; inv H.
+
+  rewrite H6 in H0. rewrite core_GHOST in H0.
+  destruct (m_phi j @ (b0,ofs0)).
+  rewrite core_NO in H0; inv H0. rewrite core_YES in H0; inv H0.
+  rewrite core_PURE in H0; inv H0.
+  rewrite core_GHOST in H0; inv H0.
+  rewrite (identity_core H3'), H8.
+  constructor; apply core_unit.
 Qed.
 
 
@@ -968,6 +997,8 @@ revert H0; case_eq (lev @ loc); intros.
 rewrite core_NO.
 destruct (access_at m loc); try destruct p; try rewrite core_NO; try rewrite core_YES; auto.
 destruct (access_at m loc); try destruct p0; try rewrite core_NO;  repeat rewrite core_YES; auto.
+destruct H1.
+destruct H2. rewrite H2. auto.
 destruct H1.
 destruct H2. rewrite H2. auto.
 Qed.
@@ -1016,6 +1047,7 @@ assert (Ha := juicy_mem_access (initial_mem m1 lev IOK1) (b',ofs')). {
   clear; if_tac; congruence.
  }
  rewrite H1 in H0. simpl in H0. contradiction.
+ rewrite H1 in H0; contradiction.
 Qed.
 
 Lemma readable_eq_after_alloc' : forall m1 m2 lo hi b lev loc IOK1 IOK2,
@@ -1065,6 +1097,7 @@ destruct loc as (b',ofs').
   unfold perm_of_sh. if_tac. if_tac; auto. rewrite if_true by auto. auto.
 
  }
+ rewrite H1 in H0. contradiction.
  rewrite H1 in H0. contradiction.
 Qed.
 
@@ -1126,6 +1159,7 @@ Proof.
   unfold perm_of_sh. if_tac. if_tac; constructor. rewrite if_true by auto; constructor.
   if_tac; constructor.
   destruct k; try constructor. apply po_join_sub_sh; eexists; eauto.
+  constructor.
   constructor.
 Qed.
 
